encrypt then decrypt then compare payloads: OK

test/main.c
@@ -4,6 +4,10 @@
 #include "EverQuic.h"
 #include "QUICTest.h"
 
+bool QUICTest_is_equal (uint8_t * b1, uint8_t * b2, uint32_t len) {
+  return (memcmp(b1, b2, len) == 0);
+}
+
 int main () {
   QUICTest_test ();
   return EXIT_SUCCESS;
